theories/memory/utp_mem_aseplog.thy
@@ -6,13 +6,13 @@ begin
 
 subsection \<open> Operators \<close>
 
-definition empty_heap :: "('s, 'h :: pam) spred" ("emp") where 
+definition empty_heap :: "('h :: pam, 's) spred" ("emp") where 
 [upred_defs]: "emp = (&hp =\<^sub>u 0)"
 
-definition sep_conj :: "('s, 'h :: sep_alg) spred \<Rightarrow> ('s, 'h) spred \<Rightarrow> ('s, 'h) spred" (infixr "\<^bold>*" 35) where
+definition sep_conj :: "('h :: sep_alg, 's) spred \<Rightarrow> ('h, 's) spred \<Rightarrow> ('h, 's) spred" (infixr "\<^bold>*" 35) where
 [upred_defs]: "(P \<^bold>* Q) = (\<^bold>\<exists> (h\<^sub>0, h\<^sub>1) \<bullet> \<guillemotleft>h\<^sub>0 ## h\<^sub>1\<guillemotright> \<and> &hp =\<^sub>u \<guillemotleft>h\<^sub>0 + h\<^sub>1\<guillemotright> \<and> P\<lbrakk>\<guillemotleft>h\<^sub>0\<guillemotright>/&hp\<rbrakk> \<and> Q\<lbrakk>\<guillemotleft>h\<^sub>1\<guillemotright>/&hp\<rbrakk>)"
 
-definition sep_impl :: "('s, 'h :: sep_alg) spred \<Rightarrow> ('s, 'h) spred \<Rightarrow> ('s, 'h) spred" (infixr "-\<^bold>*" 25) where
+definition sep_impl :: "('h :: sep_alg, 's) spred \<Rightarrow> ('h, 's) spred \<Rightarrow> ('h, 's) spred" (infixr "-\<^bold>*" 25) where
 [upred_defs]: "(P -\<^bold>* Q) = (\<^bold>\<forall> h\<^sub>0 \<bullet> \<guillemotleft>h\<^sub>0\<guillemotright> ##\<^sub>u &hp \<and> P\<lbrakk>\<guillemotleft>h\<^sub>0\<guillemotright>/&hp\<rbrakk> \<Rightarrow> Q\<lbrakk>&hp + \<guillemotleft>h\<^sub>0\<guillemotright>/&hp\<rbrakk>)"
 
 subsection \<open> Algebraic Properties \<close>
