theories/memory/utp_mem_seplog.thy
@@ -5,7 +5,7 @@ theory utp_mem_seplog
 begin
 
 definition heaplet :: "(addr, 's) uexpr \<Rightarrow> ('a::countable, 's) uexpr \<Rightarrow> 's mpred" (infix "\<^bold>\<mapsto>" 70) where
-[upred_defs]: "v \<^bold>\<mapsto> e = (dom\<^sub>u(&hp) =\<^sub>u {v \<oplus>\<^sub>p st}\<^sub>u \<and> &hp(v \<oplus>\<^sub>p st)\<^sub>a =\<^sub>u uop to_nat (e \<oplus>\<^sub>p st))"
+[upred_defs]: "v \<^bold>\<mapsto> e = (dom\<^sub>u(&hp) =\<^sub>u {v \<oplus>\<^sub>p str}\<^sub>u \<and> &hp(v \<oplus>\<^sub>p str)\<^sub>a =\<^sub>u uop to_nat (e \<oplus>\<^sub>p str))"
 
 abbreviation heaplet_min :: "(addr, 's) uexpr \<Rightarrow> ('a::countable, 's) uexpr \<Rightarrow> 's mpred" (infix "\<^bold>\<hookrightarrow>" 70) where
 "v \<^bold>\<hookrightarrow> e \<equiv> v \<^bold>\<mapsto> e \<^bold>* true"
@@ -14,7 +14,7 @@ abbreviation heaplet_ex :: "(addr, 's) uexpr \<Rightarrow> 's mpred" ("_ \<^bold
 "e \<^bold>\<mapsto> - \<equiv> (\<^bold>\<exists> v::nat \<bullet> e \<^bold>\<mapsto> \<guillemotleft>v\<guillemotright>)"
 
 lemma local_wrt_heap_lookup: 
-  "\<lbrakk> vwb_lens x; x \<sharp> e; st:x \<sharp> p \<rbrakk> \<Longrightarrow> local_wrt p (x := *e)"
+  "\<lbrakk> vwb_lens x; x \<sharp> e; str:x \<sharp> p \<rbrakk> \<Longrightarrow> local_wrt p (x := *e)"
   apply (rel_simp)
   apply (rename_tac q st hp0 hp1)
   apply (rule_tac x="hp0" in exI)
@@ -28,9 +28,9 @@ lemma allocation_noninterfering_local:
   by (rel_auto)
 
 lemma allocation_noninterfering_global:
-  "\<lbrakk> vwb_lens x; st:x \<sharp> p \<rbrakk> \<Longrightarrow> {p}x := alloc(e){p \<^bold>* &x \<^bold>\<mapsto> e}\<^sub>D"
+  "\<lbrakk> vwb_lens x; str:x \<sharp> p \<rbrakk> \<Longrightarrow> {p}x := alloc(e){p \<^bold>* &x \<^bold>\<mapsto> e}\<^sub>D"
   apply (rel_simp)
-  apply (rename_tac ok st hp ok' l)
+  apply (rename_tac ok hp st ok' l)
   apply (rule_tac x="hp" in exI)
   apply (rule_tac x="0(l \<mapsto> to_nat (\<lbrakk>e\<rbrakk>\<^sub>e (put\<^bsub>x\<^esub> st l)))\<^sub>f" in exI)
   apply (auto simp add: compat_ffun_alt_def)
@@ -61,8 +61,8 @@ lemma deallocation_global:
   done
 
 lemma lookup_global:
-  "\<lbrakk> vwb_lens x; x \<sharp> e; x \<sharp> v; st:x \<sharp> r \<rbrakk> \<Longrightarrow> 
-    {r \<^bold>* e \<^bold>\<mapsto> v} x := *e {r \<^bold>* (&st:x =\<^sub>u (v \<oplus>\<^sub>p st) \<and> e \<^bold>\<mapsto> v)}\<^sub>D"
+  "\<lbrakk> vwb_lens x; x \<sharp> e; x \<sharp> v; str:x \<sharp> r \<rbrakk> \<Longrightarrow> 
+    {r \<^bold>* e \<^bold>\<mapsto> v} x := *e {r \<^bold>* (&str:x =\<^sub>u (v \<oplus>\<^sub>p str) \<and> e \<^bold>\<mapsto> v)}\<^sub>D"
   by (rel_auto)
   
 end
